Trees.v
@@ -80,6 +80,7 @@ Inductive tree: Set :=
   | tfold: tree -> tree -> tree
   | tunfold: tree -> tree
   | tunfold_in: tree -> tree -> tree
+  | tunfold_pos_in: tree -> tree -> tree
 
   | tright: tree -> tree
   | tleft: tree -> tree
@@ -145,6 +146,7 @@ Fixpoint is_annotated_term t :=
   | tfold T t => is_annotated_type T /\ is_annotated_term t
   | tunfold t => is_annotated_term t
   | tunfold_in t1 t2 => is_annotated_term t1 /\ is_annotated_term t2
+  | tunfold_pos_in t1 t2 => is_annotated_term t1 /\ is_annotated_term t2
 
   | tleft t => is_annotated_term t
   | tright t => is_annotated_term t
@@ -311,6 +313,7 @@ Fixpoint tree_size t :=
   | tfold T t => 1 + tree_size T + tree_size t
   | tunfold t => 1 + tree_size t
   | tunfold_in t1 t2 => 1 + tree_size t1 + tree_size t2
+  | tunfold_pos_in t1 t2 => 1 + tree_size t1 + tree_size t2
 
   | tright t => 1 + tree_size t
   | tleft t => 1 + tree_size t
