LVarOperations.v
@@ -74,6 +74,7 @@ Fixpoint map_indices (k: nat) (t: tree) (f: nat -> nat) :=
   | tfold T t' => tfold (map_indices k T f) (map_indices k t' f)
   | tunfold t' => tunfold (map_indices k t' f)
   | tunfold_in t1 t2 => tunfold_in (map_indices k t1 f) (map_indices (S k) t2 f)
+  | tunfold_pos_in t1 t2 => tunfold_pos_in (map_indices k t1 f) (map_indices (S k) t2 f)
 
   | tleft t' => tleft (map_indices k t' f)
   | tright t' => tright (map_indices k t' f)
